new/proof/github_com/goose_lang/goose/model/channel/protocol/dsp/dsp.v
@@ -177,10 +177,10 @@ Qed.
  (*  send_au_slow ch v γ.(mpmc_chan_name) Φ. *)
 
 (** Endpoint sends value *)
-Lemma wp_dsp_send γ (lr_chan rl_chan : loc) (v : V) (p : iProto Σ V) Φ :
+Lemma dsp_send_au γ (lr_chan rl_chan : loc) (v : V) (p : iProto Σ V) Φ :
   £1 -∗
   #(lr_chan,rl_chan) ↣{γ} (<!> MSG v; p)%proto -∗
-  (#(lr_chan,rl_chan) ↣{γ} p -∗ Φ) -∗
+  ▷(#(lr_chan,rl_chan) ↣{γ} p -∗ Φ) -∗
   send_au_slow lr_chan v γ.(chan_lr_name) Φ.
 Proof.
   iIntros "H£ Hc HΦ".
@@ -233,7 +233,24 @@ Proof.
   - iDestruct (iProto_own_excl with "Hp Hclosel") as "[]".
 Qed.
 
-Lemma dsp_send_tele
+Lemma dsp_send (lr_chan rl_chan : loc) γ (v : V) (p : iProto Σ V) :
+  {{{ #(lr_chan,rl_chan) ↣{γ} <!> MSG v; p }}}
+    chan.send #tV #lr_chan #v
+  {{{ RET #(); #(lr_chan,rl_chan) ↣{γ} p }}}.
+Proof.
+  iIntros (Φ) "Hc HΦ".
+  iDestruct "Hc" as (?? Heq) "(#(Hcl&Hcr&HI)&Hp)".
+  rewrite to_val_unseal in Heq. simplify_eq.
+  rename lr_chan0 into lr_chan.
+  rename rl_chan0 into rl_chan.
+  iApply (chan.wp_send lr_chan v _ with "[$Hcl]").
+  iIntros "(Hlc1 & Hlc2 & _)".
+  iApply (dsp_send_au with "[$] [$Hp]").
+  { iFrame "#". done. }
+  done.
+Qed.
+
+Lemma dsp_send_tele_au
   {TT : tele} (tt:TT)
   γ (lr_chan rl_chan : loc) (v : TT → V) (P : TT → iProp Σ) (p : TT → iProto Σ V) Φ :
   £1 -∗
@@ -249,15 +266,32 @@ Proof.
     iApply iProto_le_trans;
       [iApply iProto_le_texist_intro_l|].
     by iFrame "HP". }  
-  iApply (wp_dsp_send with "H£ Hc HΦ").
+  iApply (dsp_send_au with "H£ Hc HΦ").
+Qed.
+
+Lemma dsp_send_tele
+  {TT : tele} (tt:TT)
+  (lr_chan rl_chan : loc) γ (v : TT → V) (P : TT → iProp Σ) (p : TT → iProto Σ V) :
+  {{{ #(lr_chan,rl_chan) ↣{γ} (<!.. x> MSG (v x) {{ P x }}; p x) ∗ P tt }}}
+    chan.send #tV #lr_chan #(v tt)
+  {{{ RET #(); #(lr_chan,rl_chan) ↣{γ} p tt }}}.
+Proof.
+  iIntros (Φ) "[Hc HP] HΦ".
+  iDestruct (iProto_pointsto_le _ _ _ (<!> MSG v tt; p tt)%proto with "Hc [HP]")
+    as "Hc".
+  { iIntros "!>".
+    iApply iProto_le_trans;
+      [iApply iProto_le_texist_intro_l|].
+    by iFrame "HP". }
+  by iApply (dsp_send with "Hc").
 Qed.
 
 (** Endpoint receives value *)
-Lemma wp_dsp_recv {TT:tele}
+Lemma dsp_recv_au {TT:tele}
     γ (lr_chan rl_chan : loc) (v : TT → V) (P : TT → iProp Σ) (p : TT → iProto Σ V) Φ :
   (£1 ∗ £1) -∗
   #(lr_chan,rl_chan) ↣{γ} (<?.. x> MSG (v x) {{ ▷ P x }}; p x)%proto -∗
-  (∀ x, #(lr_chan,rl_chan) ↣{γ} p x ∗ P x -∗ Φ (v x) true) -∗
+   ▷(∀ x, #(lr_chan,rl_chan) ↣{γ} p x ∗ P x -∗ Φ (v x) true) -∗
   rcv_au_slow rl_chan γ.(chan_rl_name) Φ.
 Proof.
   iIntros "H£s Hc HΦ".
@@ -372,6 +406,24 @@ Proof.
     iCombine "HP Hp" as "H".
     iMod (lc_fupd_elim_later with "H£ H") as "[HP Hp]".
     iModIntro. iRewrite "Hp". by iFrame "#∗".
+Qed.
+
+Lemma dsp_recv {TT:tele}
+    γ (lr_chan rl_chan : loc) (v : TT → V) (P : TT → iProp Σ) (p : TT → iProto Σ V) :
+  {{{ #(lr_chan,rl_chan) ↣{γ} <?.. x> MSG (v x) {{ ▷ P x }}; p x }}}
+    chan.receive #tV #rl_chan
+  {{{ x, RET (#(v x), #true); #(lr_chan,rl_chan) ↣{γ} p x ∗ P x }}}.
+Proof.
+  iIntros (Φ) "Hc HΦ".
+  iDestruct "Hc" as (?? Heq) "(#(Hcl&Hcr&HI)&Hp)".
+  rewrite to_val_unseal in Heq. simplify_eq.
+  rename lr_chan0 into lr_chan.
+  rename rl_chan0 into rl_chan.
+  iApply (chan.wp_receive _ _ with "[$Hcr]").
+  iIntros "(Hlc1 & Hlc2 & Hlc3 & Hlc4)".
+  iApply (dsp_recv_au with "[$] [$Hp]").
+  { iFrame "#". eauto. }
+  done.
 Qed.
 
 (** Endpoint closes (stops sending val) *)
